ERT/Utils/Tuple.lean
@@ -1,0 +1,114 @@
+import Mathlib.Data.Fin.Tuple.Basic
+
+def Fin.foldl_zero {α} (f: α -> Fin 0 -> α) (b: α): foldl 0 f b = b
+  := rfl
+
+theorem Fin.foldl.loop_end {α} (n: ℕ) (f: α -> Fin n -> α) (b: α): foldl.loop n f b n = b
+  := by unfold loop; simp
+theorem Fin.foldl.loop_zero {α} (f: α -> Fin 0 -> α) (b: α) (n: ℕ): foldl.loop 0 f b n = b
+  := by unfold loop; simp
+theorem Fin.foldl.loop_succ {α} (n: ℕ) (f: α -> Fin (n + 1) -> α) (b: α) (i: ℕ) (H: i < n + 1)
+  : foldl.loop (n + 1) f b i = foldl.loop n (λa i => f a i.succ) (f b i) i := if H': i < n
+  then by
+    unfold loop
+    simp only [H, ↓reduceDite, H']
+    rw [loop_succ n f _ (i + 1) (Nat.succ_lt_succ H')]
+    congr
+    rw [Nat.mod_eq_of_lt H]
+    simp only [succ_mk, Nat.cast, NatCast.natCast, ofNat'']
+    apply Fin.ext
+    simp only [Nat.mod_succ_eq_iff_lt]
+    exact Nat.succ_lt_succ H'
+  else by
+    have H' := le_antisymm (Nat.le_of_not_lt H') (Nat.le_of_succ_le_succ H);
+    cases H'
+    unfold loop
+    unfold loop
+    simp
+    rfl
+  termination_by n - i
+
+theorem Fin.foldl_succ_inner {α} (n: ℕ) (f: α -> Fin (n + 1) -> α) (b: α)
+  : foldl (n + 1) f b = foldl n (λa i => f a i.succ) (f b 0) := by
+  rw [foldl, foldl.loop_succ _ _ _ _ (by simp)]
+  congr
+
+def Fin.foldl_inner {α} (n: ℕ) (f: α -> Fin n -> α) (b: α) :=
+  match n with
+  | 0 => b
+  | n + 1 => foldl_inner n (λa i => f a i.succ) (f b 0)
+
+theorem Fin.foldl_eq_inner: @Fin.foldl α = Fin.foldl_inner := by
+  funext n
+  induction n with
+  | zero => rfl
+  | succ n I => funext f b; rw [foldl_succ_inner, foldl_inner, I]
+
+theorem Fin.foldl_succ_outer {α} (n: ℕ) (f: α -> Fin (n + 1) -> α) (b: α)
+  : foldl (n + 1) f b = f (foldl n (λa i => f a i) b) (Fin.last n)
+  := by induction n generalizing b with
+  | zero => rfl
+  | succ n I =>
+    rw [foldl_succ_inner, I, foldl_succ_inner]
+    congr
+    funext a i
+    congr
+    apply Fin.ext
+    rw [coe_eq_castSucc, coe_eq_castSucc, succ_castSucc]
+
+def Fin.foldl_outer {α} (n: ℕ) (f: α -> Fin n -> α) (b: α) :=
+  match n with
+  | 0 => b
+  | n + 1 => f (foldl_outer n (λa i => f a i) b) (Fin.last n)
+
+theorem Fin.foldl_eq_outer: @Fin.foldl α = Fin.foldl_outer := by
+  funext n
+  induction n with
+  | zero => rfl
+  | succ n I => funext f b; rw [foldl_succ_outer, foldl_outer, I]
+
+theorem sub_eq_succ_add_helper {a b c: ℕ} (H: a - b = c.succ): a = c.succ + b
+  := Nat.eq_add_of_sub_eq (Nat.le_of_lt (Nat.lt_of_sub_eq_succ H)) H
+
+theorem succ_sub_eq_succ_add_helper {a b c: ℕ} (H: a.succ - b = c.succ): a = c + b := by
+  have H := sub_eq_succ_add_helper H
+  rw [Nat.succ_add] at H
+  cases H
+  rfl
+
+def Tuple.foldl {α β} {n: ℕ} (f: α -> β -> α) (a: α) (t: Fin n -> β): α :=
+  Fin.foldl n (λa i => f a (t i)) a
+
+theorem Tuple.foldl_zero {α} (f: α -> β -> α)  (t: Fin 0 -> β) (a: α): foldl f a t = a
+  := rfl
+theorem Tuple.foldl_init {α} (f: α -> β -> α) (t: Fin (n + 1) -> β) (a: α)
+  : foldl f a t = f (foldl f a (Fin.init t)) (t n) := by
+  unfold foldl
+  rw [Fin.foldl_succ_outer]
+  congr
+  funext a i
+  simp [Fin.castSucc]
+  congr
+  apply Fin.ext
+  simp
+theorem Tuple.foldl_tail {α} (f: α -> β -> α) (t: Fin (n + 1) -> β) (b: α)
+  : foldl f b t = foldl f (f b (t 0)) (Fin.tail t) := by
+  unfold foldl
+  rw [Fin.foldl_succ_inner]
+  rfl
+
+theorem Tuple.nat_max_le_base (a: ℕ) (t: Fin n -> ℕ): a ≤ foldl Nat.max a t := by
+  induction n generalizing a with
+  | zero => rfl
+  | succ n I =>
+    simp [foldl_tail]
+    exact le_trans (le_max_left _ _) (I _ _)
+theorem Tuple.nat_max_le_ith (a: ℕ) (t: Fin n -> ℕ) (i: Fin n)
+  : t i ≤ foldl Nat.max a t := by
+  induction n generalizing a with
+  | zero => exact i.elim0
+  | succ n I =>
+    rw [foldl_tail]
+    match i with
+    | ⟨0, Hi⟩ => exact le_trans (Nat.le_max_right _ _) (nat_max_le_base _ _)
+    | ⟨i + 1, Hi⟩ => exact (I _ (Fin.tail t) ⟨i, Nat.lt_of_succ_lt_succ Hi⟩)
